Move over [is_singleton] to an [ST] function

DListRef.fst
@@ -345,8 +345,11 @@ let dlisthead_make_valid_singleton #t h =
 let g_is_singleton (#t:Type) (h:nonempty_dlisthead t) : GTot Type0 =
   g_ptr_eq (getSome h.lhead) (getSome h.ltail)
 
-let is_singleton (#t:Type) (h:nonempty_dlisthead t) : Tot bool = // TODO:FIXME: Make into ST
-  compare_addrs (getSome h.lhead) (getSome h.ltail)
+let is_singleton (#t:Type) (h:nonempty_dlisthead t) :
+  ST.ST bool
+    (requires (fun h0 -> h0 `contains` (getSome h.lhead) /\ h0 `contains` (getSome h.ltail)))
+    (ensures (fun h0 b h1 -> h0==h1 /\ (b <==> g_is_singleton h))) =
+  ptr_eq (getSome h.lhead) (getSome h.ltail)
 
 val nonempty_singleton_properties :
   #t:Type ->
